src/Running.v
@@ -1,0 +1,48 @@
+Require Import Category.
+Require Import Indexed.
+Require Import Sized.
+Require Import Success.
+Require Import Combinators.
+Require Import String.
+Require Import StringAsList.
+Require Import Ascii.
+
+Require Import Coq.Arith.Le.
+
+Inductive Singleton (A : Type) : A -> Type :=
+  MkSingleton : forall a, Singleton A a.
+
+Arguments Singleton {_}.
+Arguments MkSingleton {_}.
+
+Class Tokenizer (A : Type) : Type :=
+  MkTokenizer { _tokenize : list ascii -> list A }.
+
+Definition tokenize {A : Type} `{Tokenizer A} : list ascii -> list A := _tokenize.
+
+Arguments MkTokenizer {_}.
+
+Definition fromText {A : Type} `{Tokenizer A} (s : string) : list A :=
+  tokenize (fromString s).
+
+Instance tokAscii : Tokenizer ascii := MkTokenizer (fun x => x).
+
+Section Check.
+
+Context
+  {Tok : Type} `{Tokenizer Tok}
+  {M : Type -> Type} `{RawMonadRun M}
+  {A : Type}.
+
+Definition check : string -> [ Parser (SizedList Tok) Tok M A ] -> Type := fun s p =>
+  let tokens := (fromText s : list Tok) in
+  let n      := List.length tokens in
+  let input  := mkSizedList tokens in
+  let result := runParser (p n) (le_refl n) input in
+  let valid  := fun s => match Success.size s with | O => Some (Success.value s) | _ => None end in
+  match mapM valid (runMonad result) with
+    | Some (cons hd _) => @Singleton A hd
+    | _                => False
+  end.
+
+End Check.
